# baseURI: http://data.ashrae.org/standard223/1.0/extensions/g36
# imports: http://data.ashrae.org/standard223/1.0/extensions/g36-validation
# imports: http://data.ashrae.org/standard223/1.0/model/all
# prefix: g36

@prefix g36: <http://data.ashrae.org/standard223/1.0/extensions/g36#> .
@prefix owl: <http://www.w3.org/2002/07/owl#> .
@prefix quantitykind: <http://qudt.org/vocab/quantitykind/> .
@prefix qudt: <http://qudt.org/schema/qudt/> .
@prefix rdf: <http://www.w3.org/1999/02/22-rdf-syntax-ns#> .
@prefix rdfs: <http://www.w3.org/2000/01/rdf-schema#> .
@prefix s223: <http://data.ashrae.org/standard223#> .
@prefix sh: <http://www.w3.org/ns/shacl#> .
@prefix xsd: <http://www.w3.org/2001/XMLSchema#> .
@prefix unit: <http://qudt.org/vocab/unit/> .

<http://data.ashrae.org/standard223/1.0/extensions/g36>
  a owl:Ontology ;
  owl:imports <http://data.ashrae.org/standard223/1.0/extensions/settings> ;
  owl:imports <http://data.ashrae.org/standard223/1.0/model/all> ;
  owl:versionInfo "Created with TopBraid Composer" ;
.

#g36:AirFlowStationAnnotation
#  a sh:NodeShape ;
#  sh:rule [
#      a sh:TripleRule ;
#      sh:condition g36:AirFlowStationRule ;
# unfortunately, putting all the rules in a rule and using them in both the annotation and the constraint doesn't work too well
#      sh:object g36:AirFlowStation ;
#      sh:predicate rdf:type ;
#      sh:subject sh:this ;
#    ] ;
#  sh:targetClass s223:Sensor ;
#.
#g36:AirFlowStation
#  a sh:NodeShape, s223:Class, rdfs:Class ;
#  sh:class s223:Sensor ;
#  rdfs:label "Air Flow Station" ;
#  sh:property [
#
#    rdfs:comment "An air flow station must have an airflow property that is measured by an airflow sensor." ;
#    sh:path s223:hasProperty ;
#    sh:qualifiedMinCount 1 ;
#    sh:qualifiedValueShape [
#      sh:class s223:QuantifiableObservableProperty ;
#      sh:node [
#        sh:property [
#          sh:path qudt:hasQuantityKind ;
#          sh:hasValue quantitykind:VolumeFlowRate ;
#          sh:minCount 1;
#          sh:maxCount 1;
#        ] ;
#        sh:property [
#          sh:path s223:measuresSubstance ;
#          sh:class s223:Medium-Air ;
#          sh:minCount 1 ;
#        ];
#      ];
#    ];
#  ];
#.
g36:Damper
  a sh:NodeShape, s223:Class, rdfs:Class ;
  rdfs:label "Damper" ;
  rdfs:subClassOf s223:Damper;
  rdfs:comment "An element inserted into an air-distribution system or element of an air-distribution system permitting modification of the air resistance of the system and consequently changing the airflow rate or shutting off the airflow." ;
  sh:class s223:Damper ;
  sh:severity s223:g36;
  sh:or (
    [
      sh:property [
        sh:severity s223:g36 ;
        rdfs:comment "A damper must have at least one analog damper command property or two binary damper command property using the relation hasProperty." ;
        sh:path s223:hasProperty ;
        sh:qualifiedMinCount 1 ;
        sh:minCount 1 ;
        sh:qualifiedValueShape [
          sh:class s223:QuantifiableActuatableProperty ;
          sh:node [
            sh:property [
              sh:path qudt:hasQuantityKind ;
              sh:hasValue quantitykind:DimensionlessRatio ;
              sh:minCount 1;
              sh:maxCount 1;
            ] ;
          ];
        ] ;
      ];
    ]
    [
      sh:property [
        sh:severity s223:g36 ;
        rdfs:comment "A damper must have at least one analog damper command property or two binary damper command property using the relation hasProperty." ;
        sh:path s223:hasProperty ;
        sh:qualifiedMinCount 2 ;
        sh:minCount 2 ;
        sh:qualifiedValueShape [
          sh:class s223:EnumeratedActuatableProperty ;
        ] ;
      ];
    ]
  );
.
g36:TwoPositionDamper
  a sh:NodeShape, s223:Class, rdfs:Class ;
  rdfs:label "Two Position Damper" ;
  rdfs:subClassOf s223:Damper;
  rdfs:comment "An element inserted into an air-distribution system or element of an air-distribution system permitting modification of the air resistance of the system and consequently changing the airflow rate or shutting off the airflow. This element only has two positions: fully open and fully closed." ;
  sh:class s223:Damper ;
  sh:severity s223:g36;
  sh:property [
    sh:severity s223:g36 ;
    rdfs:comment "A Two Position Damper must have at least one open-and-close damper command property using the relation hasProperty." ;
    sh:path s223:hasProperty ;
    sh:qualifiedMinCount 1 ;
    sh:minCount 1 ;
    sh:qualifiedValueShape [
      sh:class s223:EnumeratedActuatableProperty ;
      sh:node [
        sh:property [
          sh:path s223:hasEnumerationKind;
          sh:hasValue s223:EnumerationKind-Binary;
          sh:minCount 1;
          sh:maxCount 1;
        ] ;
      ] ;
    ] ;
  ];
.
g36:HotWaterCoil
  a s223:Class, rdfs:Class, sh:NodeShape ;
  rdfs:label "HotWater/ReheatCoil" ;
  rdfs:comment "A heating element made of pipe or tube that may or may not be finned and formed into helical or serpentine shape." ;
  sh:class s223:HeatingCoil ;
  rdfs:subClassOf s223:HeatingCoil;
  sh:severity s223:g36;
  sh:property [
    sh:severity s223:g36 ;
    sh:path s223:connectedTo ;
    sh:qualifiedMinCount 1 ;
    sh:minCount 1;
    sh:qualifiedValueShape [
      sh:class g36:HotWaterValve ;
    ] ;
    rdfs:comment "The HotWaterCoil must be connectedTo a HotWaterValve using the relation connectedTo. " ;
  ] ;
.
g36:ChilledWaterCoil
  a s223:Class, rdfs:Class, sh:NodeShape ;
  rdfs:label "ChilledWaterCoil" ;
  rdfs:comment "A cooling element made of pipe or tube that may or may not be finned and formed into helical or serpentine shape." ;
  sh:class s223:CoolingCoil ;
  rdfs:subClassOf s223:CoolingCoil;
  sh:severity s223:g36;
  sh:property [
    sh:severity s223:g36 ;
    sh:path s223:connectedTo ;
    sh:qualifiedMinCount 1 ;
    sh:qualifiedValueShape [
      sh:class g36:ChilledWaterValve ;
    ] ;
    rdfs:comment "The ChilledWaterCoil must be connectedTo a ChilledWaterValve using the relation connectedTo. " ;
  ] ;
.
g36:ChilledWaterValve
  a s223:Class, rdfs:Class, sh:NodeShape ;
  rdfs:label "Chilled Water Valve" ;
  rdfs:comment "A device to regulate or stop the flow of cold fluid in a pipe or a duct by throttling." ;
  sh:class s223:Valve ;
  rdfs:subClassOf s223:Valve ;
  sh:severity s223:g36;
  sh:or (
    [
      sh:property [
        sh:severity s223:g36 ;
        rdfs:comment "A ChilledWaterValve must have at least one analog valve command property or at least two binary valve command properties.";
        sh:path s223:hasProperty ;
        sh:qualifiedMinCount 1 ;
        sh:minCount 1 ;
        sh:qualifiedValueShape [
          sh:class s223:QuantifiableActuatableProperty ;
          sh:node [
            sh:property [
              sh:path qudt:hasQuantityKind ;
              sh:hasValue quantitykind:DimensionlessRatio ;
              sh:minCount 1;
              sh:maxCount 1;
            ] ;
          ];
        ] ;
      ];
    ]
    [
      sh:property [
        sh:severity s223:g36 ;
        rdfs:comment "A ChilledWaterValve must have at least one analog valve command property or at least two binary valve command properties.";
        sh:path s223:hasProperty ;
        sh:qualifiedMinCount 2 ;
        sh:minCount 2 ;
        sh:qualifiedValueShape [
          sh:class s223:EnumeratedActuatableProperty ;
        ] ;
      ];
    ]
  );
  sh:property [
    sh:severity s223:g36 ;
    rdfs:comment "A chilled water valve must hasMedium Water-ChilledWater.";
    sh:path s223:hasMedium;
    sh:hasValue s223:Water-ChilledWater;
    sh:minCount 1;
    sh:maxCount 1;
  ];
.
g36:HotWaterValve
  a s223:Class, rdfs:Class, sh:NodeShape ;
  rdfs:label "Hot Water Valve" ;
  rdfs:comment "A device to regulate or stop the flow of hot fluid in a pipe or a duct by throttling." ;
  sh:class s223:Valve ;
  rdfs:subClassOf s223:Valve;
  sh:severity s223:g36;
  sh:or (
    [
      sh:property [
        sh:severity s223:g36 ;
        rdfs:comment "A HotWaterValve must have at least one analog valve command property or at least two binary valve command property.";
        sh:path s223:hasProperty ;
        sh:qualifiedMinCount 1 ;
        sh:minCount 1 ;
        sh:qualifiedValueShape [
          sh:class s223:QuantifiableActuatableProperty ;
          sh:node [
            sh:property [
              sh:path qudt:hasQuantityKind ;
              sh:hasValue quantitykind:DimensionlessRatio ;
              sh:minCount 1;
              sh:maxCount 1;
            ] ;
          ];
        ] ;
      ];
    ]
    [
      sh:property [
        sh:severity s223:g36 ;
        rdfs:comment "A HotWaterValve must have at least one analog valve command property or at least two binary valve command property.";
        sh:path s223:hasProperty ;
        sh:qualifiedMinCount 2 ;
        sh:minCount 2 ;
        sh:qualifiedValueShape [
          sh:class s223:EnumeratedActuatableProperty ;
        ] ;
      ];
    ]
  );

  sh:property [
    sh:severity s223:g36 ;
    rdfs:comment "A hot water valve must hasMedium Water-HotWater.";
    sh:path s223:hasMedium;
    sh:hasValue s223:Water-HotWater;
    sh:minCount 1;
    sh:maxCount 1;
  ];
.
g36:ElectricHeatingCoil
  a s223:Class, rdfs:Class, sh:NodeShape ;
  rdfs:label "Electric Heating Coil" ;
  rdfs:comment "A heating element that forms into a helical or serpentine shape and uses electricity to perform heating." ;
  sh:class s223:ResistanceHeater;
  rdfs:subClassOf s223:ResistanceHeater;
  sh:severity s223:g36;
    sh:property [
      sh:severity s223:g36 ;
      rdfs:comment "An electric heating coil must have at least one analog heating command property or two binary heating command property.";
      sh:path s223:hasProperty ;
      sh:qualifiedMinCount 1 ;
      sh:minCount 1 ;
      sh:qualifiedValueShape [
        sh:class s223:QuantifiableActuatableProperty ;
        sh:node [
          sh:property [
            sh:path qudt:hasQuantityKind ;
            sh:hasValue quantitykind:DimensionlessRatio ;
            sh:minCount 1;
            sh:maxCount 1;
          ] ;
        ];
      ] ;
    ];
.
g36:VAV
  a sh:NodeShape, s223:Class, rdfs:Class ;
  sh:class s223:SingleDuctTerminal ;
  sh:severity s223:g36;
  rdfs:subClassOf s223:SingleDuctTerminal;
  rdfs:label "VAV" ;
  rdfs:comment "An air-terminal unit assembly having one ducted air inlet and a damper for regulating the airflow rate." ;
  sh:property [
    sh:severity s223:g36 ;
    sh:path s223:contains ;
    rdfs:comment "A VAV must contain exactly one Damper." ;
    sh:qualifiedMaxCount 1 ;
    sh:minCount 1 ;
    sh:qualifiedMinCount 1 ;
    sh:qualifiedValueShape [
      sh:class g36:Damper ;
    ] ;
  ] ;
  sh:property [
    sh:severity s223:g36 ;
    sh:path s223:hasConnectionPoint;
    rdfs:comment "The VAV OutletConnectionPoint must have one discharge airflow property." ;
    rdfs:comment "This rule originally also checked connection points this may mapTo. Instead of always checking mapsTo, it would be better to have a tool that optionally applies properties to the connection points that are mapped to each other or adjacent.";
    sh:qualifiedMinCount 1;
    sh:minCount 1 ;
    sh:qualifiedValueShape [
      sh:class s223:OutletConnectionPoint;
      sh:node [
        sh:property [
          sh:path s223:hasProperty ;
          sh:qualifiedMinCount 1 ;
          sh:qualifiedValueShape [
            sh:class s223:QuantifiableObservableProperty ;
            sh:node [
              sh:property [
                sh:path qudt:hasQuantityKind ;
                sh:hasValue quantitykind:VolumeFlowRate ;
                sh:minCount 1;
                sh:maxCount 1;
              ] ;
            ] ;
          ] ;
        ];
      ];
    ];
  ] ;
.
g36:VAVWithReheat
  a s223:Class, rdfs:Class, sh:NodeShape ;
  rdfs:label "VAV with Reheat" ;
  rdfs:comment "An air-terminal unit assembly having one ducted air inlet, a damper, and a reheat coil for regulating the airflow rate and discharge air temperature." ;
  rdfs:subClassOf g36:VAV ;
  sh:severity s223:g36;
  sh:property [
    sh:severity s223:g36 ;
    sh:path s223:contains;
    rdfs:comment "The VAVWithReheat must contain a hot water coil or an electric heating coil for heating. " ;
    sh:qualifiedMinCount 1 ;
    sh:minCount 1 ;
    sh:qualifiedMaxCount 1 ;
    sh:qualifiedValueShape [
      sh:or (
        [
          sh:class g36:HotWaterCoil ;
        ]
        [
          sh:class g36:ElectricHeatingCoil ;
        ]
      );
    ] ;
  ];
  sh:property [
    sh:severity s223:g36 ;
    rdfs:comment "The VAVWithReheat OutletConnectionPoint must have a discharge air temperature property. " ;
    sh:path s223:hasConnectionPoint;
    sh:qualifiedMinCount 1;
    sh:minCount 1 ;
    sh:qualifiedValueShape [
      sh:class s223:OutletConnectionPoint;
      sh:node [
        sh:property [
          sh:path s223:hasProperty ;
          sh:qualifiedMinCount 1 ;
          sh:minCount 1 ;
          sh:qualifiedValueShape [
            sh:class s223:QuantifiableObservableProperty ;
            sh:node [
              sh:property [
                sh:path qudt:hasQuantityKind ;
                sh:hasValue quantitykind:Temperature ;
                sh:minCount 1;
                sh:maxCount 1;
              ];
            ];
          ] ;
        ];
      ];
    ];
  ] ;
.
g36:ZoneGroup
  a sh:NodeShape, s223:Class, rdfs:Class ;
  sh:class s223:Zone ;
  sh:severity s223:g36;
  rdfs:subClassOf s223:Zone;
  rdfs:label "Zone" ;
  rdfs:comment "A ZoneGroup is a grouping of zones that may be scheduled together. Zone groupings must be assigned based on rules in section 3.1.3 of Guideline 36." ;
  sh:property [
    sh:severity s223:g36 ;
    sh:path s223:hasDomain ;
    sh:hasValue s223:Domain-HVAC ;
    sh:minCount 1 ;
    rdfs:comment "A ZoneGroup must have the Domain HVAC."
  ] ;
  sh:property [
    sh:severity s223:g36 ;
    sh:path s223:contains ;
    sh:class g36:Zone;
    sh:minCount 1 ;
    rdfs:comment "A ZoneGroup must contain at least one Zone."
  ] ;
.
g36:Zone
  a sh:NodeShape, s223:Class, rdfs:Class ;
  sh:class s223:Zone ;
  sh:severity s223:g36;
  rdfs:subClassOf s223:Zone;
  rdfs:label "Zone" ;
  rdfs:comment "A Zone is a generic thermal zone, with the points required for Guideline 36 controls. It is a collection of s223:DomainSpace instances." ;
  sh:property [
    sh:severity s223:g36 ;
    sh:path s223:hasDomain ;
    rdfs:comment "A Zone must have a Domain-HVAC using the relation hasDomain. " ;
    sh:hasValue s223:Domain-HVAC ;
    sh:minCount 1 ;
  ] ;
  sh:property [
    sh:severity s223:g36 ;
    sh:path s223:hasProperty ;
    rdfs:comment "A Zone must have at least one Zone Temperature property. " ;
    sh:qualifiedMinCount 1 ;
    sh:minCount 1;
    sh:qualifiedValueShapesDisjoint true ;
    sh:qualifiedValueShape [
      sh:class s223:QuantifiableObservableProperty ;
      sh:node [
        sh:property [
          sh:path qudt:hasQuantityKind ;
          sh:hasValue quantitykind:Temperature ;
          sh:minCount 1;
          sh:maxCount 1;
        ] ;
      ] ;
    ] ;
  ] ;
  sh:property [
    sh:severity sh:Info ;
    sh:path s223:hasProperty ;
    rdfs:comment "A Zone should have a zone temperature setpoint adjustment property, if applicable. " ;
    sh:qualifiedMinCount 1 ;
    sh:minCount 1;
    sh:qualifiedValueShapesDisjoint true ;
    sh:qualifiedValueShape [
      sh:class s223:QuantifiableObservableProperty ;
      sh:node [
        sh:property [
          sh:path qudt:hasQuantityKind ;
          sh:hasValue quantitykind:Temperature ;
          sh:minCount 1;
          sh:maxCount 1;
        ] ;
        sh:property [
          sh:path s223:hasAspect ;
          sh:hasValue s223:Dimensioned-Delta ;
          sh:minCount 1;
          sh:maxCount 1;
        ] ;
      ] ;
    ] ;
  ] ;
  sh:property [
    sh:severity sh:Info ;
    sh:path s223:hasProperty ;
    rdfs:comment "A Zone should have at a zone CO2 concentration property, if applicable control is used. " ;
    sh:qualifiedMinCount 1 ;
    sh:minCount 1;
    sh:qualifiedValueShape [
      sh:class s223:QuantifiableObservableProperty ;
      sh:node [
        sh:property [
          sh:path qudt:hasQuantityKind ;
          sh:hasValue quantitykind:DimensionlessRatio ;
          sh:minCount 1;
          sh:maxCount 1;
        ] ;
        sh:property [
          sh:path s223:ofSubstance ;
          sh:hasValue s223:Substance-CO2 ;
          sh:minCount 1;
          sh:maxCount 1;
        ] ;
      ] ;
    ] ;
  ] ;
  sh:property [
    sh:severity sh:Info ;
    sh:path s223:hasProperty ;
    rdfs:comment "A Zone should have at least one binary zone occupancy property. " ;
    sh:qualifiedMinCount 1 ;
    sh:minCount 1;
    sh:qualifiedValueShape [
      sh:class s223:EnumeratedObservableProperty;
      sh:node [
        sh:property [
          sh:path s223:hasEnumerationKind;
          sh:hasValue s223:EnumerationKind-Occupancy;
          sh:minCount 1;
          sh:maxCount 1;
        ] ;
      ] ;
    ] ;
  ] ;
  sh:property [
    sh:severity sh:Info ;
    sh:path s223:hasProperty ;
    rdfs:comment "A Zone should have at least one window switch OnOff property." ;
    sh:qualifiedMinCount 1 ;
    sh:minCount 1;
    sh:qualifiedValueShape [
      sh:class s223:EnumeratedObservableProperty;
      sh:node [
        sh:property [
          sh:path s223:hasEnumerationKind;
          sh:hasValue s223:EnumerationKind-OnOff;
          sh:minCount 1;
          sh:maxCount 1;
        ] ;
        sh:property [
          rdfs:comment "Property must be measured at a window" ;
          sh:path [
            sh:alternativePath (
                (
                  [ sh:inversePath s223:observes ]
                  s223:hasMeasurementLocation
                )
                [ sh:inversePath s223:hasProperty ]
              )
            ] ;
          sh:class s223:Window ;
        ] ;
      ] ;
    ] ;
  ] ;
  sh:property [
    sh:severity sh:Info ;
    sh:path s223:hasProperty ;
    rdfs:comment "A Zone should have at least one zone thermostat override switch property. " ;
    sh:qualifiedMinCount 1 ;
    sh:minCount 1;
    sh:qualifiedValueShape [
      sh:class s223:EnumeratedObservableProperty;
      sh:node [
        sh:property [
          sh:path s223:hasEnumerationKind;
          sh:hasValue s223:EnumerationKind-Override;
          sh:minCount 1;
          sh:maxCount 1;
        ] ;
      ] ;
    ] ;
  ] ;
.

g36:Fan
  a sh:NodeShape, rdfs:Class, s223:Class ;
  sh:class s223:Fan ;
  sh:severity s223:g36;
  rdfs:subClassOf s223:Fan;
  rdfs:label "Fan" ;
  rdfs:comment "A machine used to create flow within a gas such as air." ;
  sh:property [
    sh:severity s223:g36 ;
    rdfs:comment "A Fan must have at least one Start/Stop command." ;
    sh:path s223:hasProperty ;
    sh:qualifiedMinCount 1 ;
    sh:minCount 1;
    sh:qualifiedValueShape [
      sh:class s223:EnumeratedActuatableProperty ;
      sh:node [
        sh:property [
          sh:path s223:hasEnumerationKind;
          sh:hasValue s223:EnumerationKind-OnOff;
          sh:minCount 1;
          sh:maxCount 1;
        ] ;
      ] ;
    ] ;
  ] ;
.

g36:FanPoweredTerminal
  a sh:NodeShape, s223:Class, rdfs:Class ;
  sh:class s223:FanPoweredTerminal ;
  rdfs:subClassOf s223:FanPoweredTerminal;
  sh:severity s223:g36;
  rdfs:label "FanPoweredTerminal" ;
  rdfs:comment "An air terminal containing a fan. Airflow may pass through or be parallel to the fan. These units may also have supplemental heating or cooling." ;
  sh:property [
    sh:severity s223:g36 ;
    sh:path s223:contains ;
    rdfs:comment "A FanPoweredTerminal must have exactly one Damper using the relation contains." ;
    sh:qualifiedMaxCount 1 ;
    sh:qualifiedMinCount 1 ;
    sh:minCount 1;
    sh:qualifiedValueShape [
      sh:class g36:Damper ;
    ] ;
  ] ;
  sh:property [
    sh:severity s223:g36 ;
    sh:path s223:contains ;
    rdfs:comment "A FanPoweredTerminal must have exactly one Fan or FanWithVFD using the relation contains." ;
    sh:qualifiedMaxCount 1 ;
    sh:qualifiedMinCount 1 ;
    sh:minCount 1 ;
    sh:qualifiedValueShape [
      sh:or (
        [
          sh:class g36:Fan ;
        ]
        [
          sh:class g36:FanWithVFD ;
        ]
      );
    ] ;
  ] ;
  sh:property [
    sh:severity s223:g36 ;
    rdfs:comment "The FanPoweredTerminal InletConnectionPoint must have a supply airflow property." ;
    sh:path s223:hasConnectionPoint;
    sh:qualifiedMinCount 1;
    sh:minCount 1 ;
    sh:qualifiedValueShape [
      sh:class s223:InletConnectionPoint;
      sh:node [
        sh:property [
          sh:path s223:hasProperty ;
          sh:qualifiedMinCount 1 ;
          sh:qualifiedValueShape [
            sh:class s223:QuantifiableObservableProperty ;
            sh:node [
              sh:property [
                sh:path qudt:hasQuantityKind ;
                sh:hasValue quantitykind:VolumeFlowRate ;
                sh:minCount 1;
                sh:maxCount 1;
              ] ;
            ];
          ];
        ];
      ];
    ];
  ];

  sh:property [
    sh:severity s223:g36 ;
    sh:path s223:contains;
    rdfs:comment "A FanPoweredTerminal must contain a hot water coil or an electric heating coil for heating." ;
    sh:qualifiedMinCount 1 ;
    sh:minCount 1 ;
    sh:qualifiedMaxCount 1 ;
    sh:qualifiedValueShape [
      sh:or (
        [
          sh:class g36:HotWaterCoil ;
        ]
        [
          sh:class g36:ElectricHeatingCoil ;
        ]
      );
    ] ;
  ];

  sh:property [
    sh:severity s223:g36 ;
    rdfs:comment "The FanPoweredTerminal OutletConnectionPoint must have a discharge air temperature property. " ;
    sh:path s223:hasConnectionPoint;
    sh:qualifiedMinCount 1;
    sh:minCount 1 ;
    sh:qualifiedValueShape [
      sh:class s223:OutletConnectionPoint;
      sh:node [
        sh:property [
          sh:path s223:hasProperty ;
          sh:qualifiedMinCount 1 ;
          sh:qualifiedValueShape [
            sh:class s223:QuantifiableObservableProperty ;
            sh:node [
              sh:property [
                sh:path qudt:hasQuantityKind ;
                sh:hasValue quantitykind:Temperature ;
                sh:minCount 1;
                sh:maxCount 1;
              ];
            ];
          ] ;
        ];
      ];
    ];
  ] ;
.
g36:DualDuctTerminalWithInletSensors
  a s223:Class, rdfs:Class, sh:NodeShape ;
  rdfs:label "DualDuctTerminalWithInletSensors" ;
  rdfs:comment "A dual duct air terminal mixes two independent sources of primary air. This terminal uses two inlet sensors." ;
  sh:class s223:DualDuctTerminal ;
  rdfs:subClassOf s223:DualDuctTerminal;
  sh:severity s223:g36;
  sh:property [
    sh:severity s223:g36 ;
    rdfs:comment "DualDuctTerminalWithInletSensors shall contain 2 dampers" ;
    sh:path s223:contains ;
    sh:minCount 2 ;
    sh:maxCount 2 ;
    sh:class g36:Damper ;
  ] ;
  sh:property [
    sh:severity s223:g36 ;
    rdfs:comment "DualDuctTerminalWithInletSensors shall contain 1 damper that has the Role Heating." ;
    sh:path s223:contains ;
    sh:qualifiedMinCount 1 ;
    sh:minCount 1 ;
    sh:qualifiedValueShape [
      sh:class g36:Damper ;
      sh:node [
        sh:property [
          sh:path s223:hasRole;
          sh:qualifiedMinCount 1 ;
          sh:minCount 1 ;
          sh:qualifiedValueShape [
            sh:hasValue s223:Role-Heating ;
          ];
        ] ;
      ] ;
    ] ;
  ] ;
  sh:property [
    sh:severity s223:g36 ;
    rdfs:comment "DualDuctTerminalWithInletSensors shall contain 1 damper that has the Role Cooling." ;
    sh:path s223:contains ;
    sh:qualifiedMinCount 1 ;
    sh:minCount 1 ;
    sh:qualifiedValueShape [
      sh:class g36:Damper ;
      sh:node [
        sh:property [
          sh:path s223:hasRole ;
          sh:qualifiedMinCount 1 ;
          sh:minCount 1 ;
          sh:qualifiedValueShape [
            sh:hasValue s223:Role-Cooling ;
          ];
        ] ;
      ] ;
    ] ;
  ] ;
  sh:property [
    sh:severity s223:g36 ;
    rdfs:comment "The DualDuctTerminalWithInletSensors InletConnectionPoint must have a cooling supply airflow property." ;
    sh:path s223:hasConnectionPoint;
    sh:qualifiedMinCount 1;
    sh:qualifiedValueShape [
      sh:class s223:InletConnectionPoint;
      sh:node [
        sh:property [
          sh:path s223:hasProperty ;
          sh:qualifiedMinCount 1 ;
          sh:minCount 1 ;
          sh:qualifiedValueShape [
            sh:class s223:QuantifiableObservableProperty ;
            sh:node [
              sh:property [
                sh:path qudt:hasQuantityKind ;
                sh:hasValue quantitykind:VolumeFlowRate ;
                sh:minCount 1;
                sh:maxCount 1;
              ] ;
              sh:property [
                sh:path s223:hasAspect;
                sh:qualifiedMinCount 1 ;
                sh:minCount 1 ;
                sh:qualifiedValueShape [
                  sh:hasValue s223:Role-Cooling ;
                ];
              ] ;
            ];
          ];
        ];
      ];
    ];
  ];

  sh:property [
    sh:severity s223:g36 ;
    rdfs:comment "The DualDuctTerminalWithInletSensors InletConnectionPoint must have a heating supply airflow property." ;
    sh:path s223:hasConnectionPoint;
    sh:qualifiedMinCount 1;
    sh:minCount 1 ;
    sh:qualifiedValueShape [
      sh:class s223:InletConnectionPoint;
      sh:node [
        sh:property [
          sh:path s223:hasProperty ;
          sh:qualifiedMinCount 1 ;
          sh:minCount 1 ;
          sh:qualifiedValueShape [
            sh:class s223:QuantifiableObservableProperty ;
            sh:node [
              sh:property [
                sh:path qudt:hasQuantityKind ;
                sh:hasValue quantitykind:VolumeFlowRate ;
                sh:minCount 1;
                sh:maxCount 1;
              ] ;
              sh:property [
                sh:path s223:hasAspect;
                sh:qualifiedMinCount 1 ;
                sh:minCount 1 ;
                sh:qualifiedValueShape [
                  sh:hasValue s223:Role-Heating ;
                ];
              ] ;
            ];
          ];
        ];
      ];
    ];
  ];
.

g36:DualDuctTerminalWithDischargeSensor
  a s223:Class, rdfs:Class, sh:NodeShape ;
  rdfs:label "DualDuctTerminalWithDischargeSensor" ;
  rdfs:comment "A dual duct air terminal mixes two independent sources of primary air. This terminal uses one discharge sensor." ;
  sh:class s223:DualDuctTerminal ;
  rdfs:subClassOf s223:DualDuctTerminal;
  sh:severity s223:g36;
  sh:property [
    sh:severity s223:g36 ;
    rdfs:comment "DualDuctTerminalWithDischargeSensor shall contain 2 dampers" ;
    sh:path s223:contains ;
    sh:minCount 2 ;
    sh:maxCount 2 ;
    sh:qualifiedValueShape[
      sh:class g36:Damper ;
    ];
  ] ;
  sh:property [
    sh:severity s223:g36 ;
    rdfs:comment "In DualDuctTerminalWithDischargeSensor, one Damper has Role Heating" ;
    sh:path s223:contains ;
    sh:qualifiedMinCount 1 ;
    sh:minCount 1 ;
    sh:qualifiedValueShape [
      sh:class g36:Damper ;
      sh:node [
        sh:property [
          sh:path s223:hasRole ;
          sh:qualifiedMinCount 1 ;
          sh:minCount 1 ;
          sh:qualifiedValueShape [
            sh:hasValue s223:Role-Heating ;
          ];
        ] ;
      ] ;
    ] ;
  ] ;
  sh:property [
    sh:severity s223:g36 ;
    rdfs:comment "In DualDuctTerminalWithDischargeSensor, one Damper has Role Cooling" ;
    sh:path s223:contains ;
    sh:qualifiedMinCount 1 ;
    sh:minCount 1 ;
    sh:qualifiedValueShape [
      sh:class g36:Damper ;
      sh:node [
        sh:property [
          sh:path s223:hasRole ;
          sh:qualifiedMinCount 1 ;
          sh:minCount 1 ;
          sh:qualifiedValueShape [
            sh:hasValue s223:Role-Cooling ;
          ];
        ] ;
      ] ;
    ] ;
  ] ;

  sh:property [
    sh:severity s223:g36 ;
    sh:path s223:hasConnectionPoint;
    rdfs:comment "The DualDuctTerminalWithDischargeSensor OutletConnectionPoint must have one discharge airflow property.";
    sh:qualifiedMinCount 1;
    sh:minCount 1 ;
    sh:qualifiedValueShape [
      sh:class s223:OutletConnectionPoint;
      sh:node [
        sh:property [
          sh:path s223:hasProperty ;
          sh:qualifiedMinCount 1 ;
          sh:minCount 1 ;
          sh:qualifiedValueShape [
            sh:class s223:QuantifiableObservableProperty ;
            sh:node [
              sh:property [
                sh:path qudt:hasQuantityKind ;
                sh:hasValue quantitykind:VolumeFlowRate ;
                sh:minCount 1;
                sh:maxCount 1;
              ] ;
            ] ;
          ] ;
        ];
      ];
    ];
  ] ;
.
g36:FanWithVFD
  a sh:NodeShape, s223:Class, rdfs:Class;
  sh:class s223:Fan ;
  sh:severity s223:g36;
  rdfs:label "FanWithVFD" ;
  rdfs:comment "A machine used to create flow within a gas such as air. This machine can be controlled to vary in speed." ;
  rdfs:subClassOf g36:Fan ;
  sh:property [
    sh:severity s223:g36 ;
    rdfs:comment "A fan with VFD must have a fan speed command" ;
    sh:path s223:hasProperty ;
    sh:qualifiedMinCount 1 ;
    sh:minCount 1 ;
    sh:qualifiedValueShape [
      sh:class s223:QuantifiableActuatableProperty ;
      sh:node [
        sh:property [
          sh:path qudt:hasQuantityKind ;
          sh:value quantitykind:DimensionlessRatio ;
          sh:minCount 1;
          sh:maxCount 1;
        ] ;
      ] ;
    ] ;
  ] ;
.

g36:Filter
  a sh:NodeShape, rdfs:Class, s223:Class;
  rdfs:label "Filter" ;
  rdfs:comment "A device that removes particulates from gasses such as air." ;
  sh:severity s223:g36;
  rdfs:subClassOf s223:AirFilter ;
  sh:class s223:AirFilter ;
.

g36:DualFanDualDuctAirHandlingUnit
  a sh:NodeShape, rdfs:Class, s223:Class ;
  rdfs:label "DualFanDualDuctAirHandlingUnit" ;
  rdfs:comment "DualFanDualDuctAirHandlingUnit" ;
  sh:severity s223:g36;
  rdfs:subClassOf s223:AirHandlingUnit;
  sh:class s223:AirHandlingUnit ;
  sh:property [
    sh:severity s223:g36 ;
    rdfs:comment "The DualFanDualDuctAirHandlingUnit must contain at least one supply fan with a VFD that has the role Supply." ;
    sh:path s223:contains ;
    sh:qualifiedMinCount 1 ;
    sh:minCount 1 ;
    sh:qualifiedValueShape [
      sh:class g36:FanWithVFD ;
      sh:node [
        sh:property [
          sh:path s223:hasRole ;
          sh:hasValue s223:Role-Supply ;
        ] ;
      ] ;
    ] ;
  ];
  sh:property [
    sh:severity s223:g36 ;
    rdfs:comment "The DualFanDualDuctAirHandlingUnit must contain at least one HotWaterCoil or an ElectricHeatingCoil for heating." ;
    sh:path s223:contains;
    sh:qualifiedMinCount 1 ;
    sh:minCount 1 ;
    sh:qualifiedValueShape [
      sh:or (
        [
          sh:class g36:HotWaterCoil ;
        ]
        [
          sh:class g36:ElectricHeatingCoil ;
        ]
      );
    ] ;
  ];
  sh:property [
    sh:severity s223:g36 ;
    rdfs:comment "A DualFanDualDuctAirHandlingUnit OutletConnectionPoint must have a supply duct static pressure property." ;
    sh:path s223:hasConnectionPoint;
    sh:qualifiedMinCount 1;
    sh:minCount 1 ;
    sh:qualifiedValueShape [
      sh:class s223:OutletConnectionPoint;
      sh:node [
        sh:property [
          sh:path s223:hasProperty ;
          sh:qualifiedMinCount 1 ;
          sh:minCount 1 ;
          sh:qualifiedValueShape [
            sh:class s223:QuantifiableObservableProperty ;
            sh:node [
              sh:property [
                sh:path qudt:hasQuantityKind ;
                sh:hasValue quantitykind:Pressure ;
                sh:minCount 1;
                sh:maxCount 1;
              ];
              sh:property [
                sh:path s223:hasAspect ;
                sh:hasValue s223:Role-Supply ;
                sh:minCount 1;
                sh:maxCount 1;
              ];
            ];
          ] ;
        ];
      ];
    ];
  ];
  sh:property [
    sh:severity s223:g36 ;
    rdfs:comment "A DualFanDualDuctAirHandlingUnit OutletConnectionPoint must have a supply air temperature property." ;
    sh:path s223:hasConnectionPoint;
    sh:qualifiedMinCount 1;
    sh:minCount 1 ;
    sh:qualifiedValueShape [
      sh:class s223:OutletConnectionPoint;
      sh:node [
        sh:property [
          sh:path s223:hasProperty ;
          sh:qualifiedMinCount 1 ;
          sh:minCount 1 ;
          sh:qualifiedValueShape [
            sh:class s223:QuantifiableObservableProperty ;
            sh:node [
              sh:property [
                sh:path qudt:hasQuantityKind ;
                sh:hasValue quantitykind:Temperature ;
                sh:minCount 1;
                sh:maxCount 1;
              ];
              sh:property [
                sh:path s223:hasAspect ;
                sh:hasValue s223:Role-Supply ;
                sh:minCount 1;
                sh:maxCount 1;
              ];
            ];
          ] ;
        ];
      ];
    ];
  ] ;
.
g36:SingleZoneVAVAirHandlingUnit
  a sh:NodeShape, rdfs:Class, s223:Class ;
  sh:severity s223:g36;
  sh:class s223:AirHandlingUnit ;
  rdfs:subClassOf s223:AirHandlingUnit;
  rdfs:label "SingleZoneVAVAirHandlingUnit" ;
  rdfs:comment "An assembly consisting of sections containing a fan or fans and other necessary equipment to perform one or more of the following functions: circulating, filtration, heating, cooling, heat recovery, humidifying, dehumidifying, and mixing of air. It is usually connected to an air-distribution system. This air handling unit that serves one zone only." ;
  sh:property [
    sh:severity s223:g36 ;
    rdfs:comment "The SingleZoneVAVAirHandlingUnit must contain at least one supply fan with a VFD that has the role Supply." ;
    sh:path s223:contains ;
    sh:qualifiedMinCount 1 ;
    sh:minCount 1 ;
    sh:qualifiedValueShape [
      sh:class g36:FanWithVFD ;
      sh:node [
        sh:property [
          sh:path s223:hasRole ;
          sh:hasValue s223:Role-Supply ;
        ] ;
      ] ;
    ] ;
  ];
  sh:property [
    sh:severity s223:g36 ;
    rdfs:comment "The SingleZoneVAVAirHandlingUnit must contain at least one HotWaterCoil or an ElectricHeatingCoil for heating." ;
    sh:path s223:contains;
    sh:qualifiedMinCount 1 ;
    sh:minCount 1;
    sh:qualifiedValueShape [
      sh:or (
        [
          sh:class g36:HotWaterCoil ;
        ]
        [
          sh:class g36:ElectricHeatingCoil ;
        ]
      );
    ] ;
  ];
  sh:property [
    sh:severity s223:g36 ;
    rdfs:comment "A SingleZoneVAVAirHandlingUnit OutletConnectionPoint must have a supply air temperature property." ;
    sh:path s223:hasConnectionPoint;
    sh:qualifiedMinCount 1;
    sh:minCount 1;
    sh:qualifiedValueShape [
      sh:class s223:OutletConnectionPoint;
      sh:node [
        sh:property [
          sh:path s223:hasProperty ;
          sh:qualifiedMinCount 1 ;
          sh:minCount 1;
          sh:qualifiedValueShape [
            sh:class s223:QuantifiableObservableProperty ;
            sh:node [
              sh:property [
                sh:path qudt:hasQuantityKind ;
                sh:hasValue quantitykind:Temperature ;
                sh:minCount 1;
                sh:maxCount 1;
              ];
              sh:property [
                sh:path s223:hasAspect ;
                sh:hasValue s223:Role-Supply ;
                sh:minCount 1;
                sh:maxCount 1;
              ];
            ];
          ] ;
        ];
      ];
    ];
  ] ;
  sh:property [
    sh:severity s223:g36 ;
    rdfs:comment "The SingleZoneVAVAirHandlingUnit must have at least one outdoor air damper." ;
    sh:path s223:contains ;
    sh:qualifiedMinCount 1 ;
    sh:minCount 1;
    sh:qualifiedValueShape [
      sh:class g36:Damper ;
      sh:node [
        sh:property [
          sh:path s223:hasRole;
          sh:qualifiedMinCount 1;
          sh:minCount 1;
          sh:qualifiedValueShape [
            sh:hasValue s223:Role-Outside;
          ];
        ];
      ];
    ];
  ];
  sh:property [
    sh:severity s223:g36 ;
    rdfs:comment "The SingleZoneVAVAirHandlingUnit must have at least one return air damper." ;
    sh:path s223:contains ;
    sh:qualifiedMinCount 1 ;
    sh:minCount 1;
    sh:qualifiedValueShape [
      sh:class g36:Damper ;
      sh:node [
        sh:property [
          sh:path s223:hasRole;
          sh:qualifiedMinCount 1;
          sh:minCount 1;
          sh:qualifiedValueShape [
            sh:hasValue s223:Role-Return;
          ];
        ];
      ];
    ];
  ];
  sh:property [
    sh:severity s223:g36 ;
    sh:path s223:contains;
    rdfs:comment "The  SingleZoneVAVAirHandlingUnit must contain at least one ChilledWaterCoil for cooling." ;
    sh:qualifiedMinCount 1 ;
    sh:minCount 1;
    sh:qualifiedValueShape [
      sh:class g36:ChilledWaterCoil ;
    ] ;
  ];
.
g36:SingleZoneVAVAirHandlingUnit-AllPoints
  a sh:NodeShape, rdfs:Class, s223:Class ;
  sh:severity s223:g36;
  sh:class s223:AirHandlingUnit ;
  rdfs:subClassOf g36:SingleZoneVAVAirHandlingUnit;
  rdfs:label "SingleZoneVAVAirHandlingUnit" ;
  rdfs:comment "An assembly consisting of sections containing a fan or fans and other necessary equipment to perform one or more of the following functions: circulating, filtration, heating, cooling, heat recovery, humidifying, dehumidifying, and mixing of air. It is usually connected to an air-distribution system. This air handling unit that serves one zone only." ;
  sh:property [
    sh:severity s223:g36 ;
    rdfs:comment "In the case where the SingleZoneVAVAirHandlingUnit has relief dampers but no relief fan, a modulating damper should be contained." ;
    sh:path s223:contains ;
    sh:qualifiedMinCount 1 ;
    sh:minCount 1;
    sh:qualifiedValueShape [
      sh:class g36:Damper ;
      sh:node [
        sh:property [
          sh:path s223:hasRole;
          sh:hasValue s223:Role-Relief;
          sh:minCount 1;
          sh:maxCount 1;
        ];
      ];
    ] ;
  ];
  sh:property [
    sh:severity s223:g36 ;
    rdfs:comment "For the case where the SingleZoneVAVAirHandlingUnit has both a relief air damper and a relief fan, a two position relief damper and relief fan should be contained." ;
    sh:path s223:contains ;
    sh:qualifiedMinCount 1 ;
    sh:minCount 1;
    sh:qualifiedMaxCount 1 ;
    sh:qualifiedValueShape [
      sh:class g36:TwoPositionDamper ;
      sh:node [
        sh:property [
          sh:path s223:hasRole;
          sh:qualifiedMinCount 1;
          sh:qualifiedValueShape [
            sh:hasValue s223:Role-Relief;
          ];
        ];
      ];
    ];
  ];
  sh:property [
    sh:severity s223:g36 ;
    rdfs:comment "For the case where the SingleZoneVAVAirHandlingUnit has both a relief air damper and a relief fan, the SingleZoneVAVAirHandlingUnit must indeed have a relief fan." ;
    sh:path s223:contains ;
    sh:qualifiedMinCount 1 ;
    sh:minCount 1;
    sh:qualifiedMaxCount 1 ;
    sh:qualifiedValueShape [
      sh:class g36:FanWithVFD ;
      sh:node [
        sh:property [
          sh:path s223:hasRole;
          sh:qualifiedMinCount 1;
          sh:minCount 1 ;
          sh:qualifiedValueShape [
            sh:hasValue s223:Role-Relief;
          ];
        ];
      ];
    ];
  ];
  sh:property [
    sh:severity s223:g36 ;
    rdfs:comment "For the case where the SingleZoneVAVAirHandlingUnit has both a relief air damper and a relief fan, the SingleZoneVAVAirHandlingUnit must be connectedTo at least one VAV, which connectedTo at least one HVAC DomainSpace, which is contained by at least one Zone, which has a building static pressure property." ;
    sh:path (s223:connectedTo s223:connectedTo [sh:inversePath s223:contains;] s223:hasProperty) ;
    sh:qualifiedMinCount 1 ;
    sh:minCount 1;
    sh:qualifiedValueShape [
      sh:class s223:QuantifiableObservableProperty ;
      sh:node [
        sh:property [
          sh:path qudt:hasQuantityKind ;
          sh:hasValue quantitykind:Pressure ;
          sh:minCount 1;
          sh:maxCount 1;
        ];
      ];
    ];
  ];
  sh:property [
    rdfs:comment "For the case where the SingleZoneVAVAirHandlingUnit has a return fan, the SingleZoneVAVAirHandlingUnit must indeed contain a return fan." ;
    sh:severity s223:g36 ;
    sh:path s223:contains ;
    sh:qualifiedMinCount 1 ;
    sh:minCount 1;
    sh:qualifiedValueShape [
      sh:class g36:FanWithVFD ;
      sh:node [
        sh:property [
          sh:path s223:hasRole ;
          sh:hasValue s223:Role-Return ;
          sh:minCount 1 ;
        ] ;
      ] ;
    ] ;
  ] ;
  sh:property [
    sh:severity s223:g36 ;
    rdfs:comment "For the case where the SingleZoneVAVAirHandlingUnit has a return fan, the SingleZoneVAVAirHandlingUnit must contain an exhaust air damper with either an analog or two-position damper command property." ;
    sh:path s223:contains ;
    sh:qualifiedMinCount 1 ;
    sh:minCount 1;
    sh:qualifiedValueShape [
      sh:or (
        [
          sh:class g36:Damper ;
        ]
        [
          sh:class g36:TwoPositionDamper ;
        ]
      );
      sh:node [
        sh:property [
          sh:path s223:hasRole;
          sh:hasValue s223:Role-Exhaust;
          sh:minCount 1;
          sh:maxCount 1;
        ];
      ];
    ] ;
  ] ;
.

g36:MultiZoneVAVAirHandlingUnit
  a sh:NodeShape, rdfs:Class, s223:Class ;
  sh:severity s223:g36;
  sh:class s223:AirHandlingUnit ;
  rdfs:subClassOf s223:AirHandlingUnit;
  rdfs:label "MultiZoneVAVAirHandlingUnit" ;
  rdfs:comment "An assembly consisting of sections containing a fan or fans and other necessary equipment to perform one or more of the following functions: circulating, filtration, heating, cooling, heat recovery, humidifying, dehumidifying, and mixing of air. It is usually connected to an air-distribution system. This air handling unit serves multiple zones." ;
  sh:property [
    sh:severity s223:g36 ;
    rdfs:comment "One MultiZoneVAVAirHandlingUnit InletConnectionPoint must have at least one return air temperature property. " ;
    sh:path s223:hasConnectionPoint;
    sh:qualifiedMinCount 1;
    sh:minCount 1 ;
    sh:qualifiedValueShape [
      sh:class s223:InletConnectionPoint;
      sh:node [
        sh:property [
          sh:path s223:hasProperty ;
          sh:qualifiedMinCount 1 ;
          sh:minCount 1;
          sh:qualifiedValueShape [
            sh:class s223:QuantifiableObservableProperty ;
            sh:node [
              sh:property [
                sh:path qudt:hasQuantityKind ;
                sh:hasValue quantitykind:Temperature ;
                sh:minCount 1;
                sh:maxCount 1;
              ];
              sh:property [
                sh:path s223:hasAspect ;
                sh:hasValue s223:Role-Return ;
                sh:minCount 1;
                sh:maxCount 1;
              ];
            ];
          ];
        ] ;
      ];
    ];
  ];
  sh:property [
    sh:severity s223:g36 ;
    rdfs:comment "One MultiZoneVAVAirHandlingUnit InletConnectionPoint must have at least one outdoor air temperature property. " ;
    sh:path s223:hasConnectionPoint;
    sh:qualifiedMinCount 1;
    sh:qualifiedValueShape [
      sh:class s223:InletConnectionPoint;
      sh:node [
        sh:property [
          sh:path s223:hasProperty ;
          sh:qualifiedMinCount 1 ;
          sh:minCount 1;
          sh:qualifiedValueShape [
            sh:class s223:QuantifiableObservableProperty ;
            sh:node [
              sh:property [
                sh:path qudt:hasQuantityKind ;
                sh:hasValue quantitykind:Temperature ;
                sh:minCount 1;
                sh:maxCount 1;
              ];
              sh:property [
                sh:path s223:hasAspect ;
                sh:hasValue s223:Role-Outside ;
                sh:minCount 1;
                sh:maxCount 1;
              ];
            ];
          ];
        ] ;
      ];
    ];
  ];
  sh:property [
    sh:severity s223:g36 ;
    rdfs:comment "The MultiZoneVAVAirHandlingUnit must contain a Supply Fan with a VFD that has the role Supply" ;
    sh:path s223:contains ;
    sh:qualifiedMinCount 1 ;
    sh:minCount 1;
    sh:qualifiedValueShape [
      sh:class g36:FanWithVFD ;
      sh:node [
        sh:property [
          sh:path s223:hasRole ;
          sh:hasValue s223:Role-Supply ;
        ] ;
      ] ;
    ] ;
  ] ;
  sh:property [
    sh:severity s223:g36 ;
    rdfs:comment "One MultiZoneVAVAirHandlingUnit OutletConnectionPoint must have a supply air temperature property. " ;
    sh:path s223:hasConnectionPoint;
    sh:qualifiedMinCount 1;
    sh:minCount 1;
    sh:qualifiedValueShape [
      sh:class s223:OutletConnectionPoint;
      sh:node [
        sh:property [
          sh:path s223:hasProperty ;
          sh:qualifiedMinCount 1 ;
          sh:minCount 1;
          sh:qualifiedValueShape [
            sh:class s223:QuantifiableObservableProperty ;
            sh:node [
              sh:property [
                sh:path qudt:hasQuantityKind ;
                sh:hasValue quantitykind:Temperature ;
                sh:minCount 1;
                sh:maxCount 1;
              ];
              sh:property [
                sh:path s223:hasAspect ;
                sh:hasValue s223:Role-Supply ;
                sh:minCount 1;
                sh:maxCount 1;
              ];
            ];
          ] ;
        ];
      ];
    ];
  ] ;
  sh:property [
    sh:severity s223:g36 ;
    rdfs:comment "The MultiZoneVAVAirHandlingUnit OutletConnectionPoint must have a supply duct static pressure property. " ;
    sh:path s223:hasConnectionPoint;
    sh:qualifiedMinCount 1;
    sh:qualifiedValueShape [
      sh:class s223:OutletConnectionPoint;
      sh:node [
        sh:property [
          sh:path s223:hasProperty ;
          sh:qualifiedMinCount 1 ;
          sh:minCount 1;
          sh:qualifiedValueShape [
            sh:class s223:QuantifiableObservableProperty ;
            sh:node [
              sh:property [
                sh:path qudt:hasQuantityKind ;
                sh:hasValue quantitykind:Pressure ;
                sh:minCount 1;
                sh:maxCount 1;
              ];
              sh:property [
                sh:path s223:hasAspect ;
                sh:hasValue s223:Role-Supply ;
                sh:minCount 1;
                sh:maxCount 1;
              ];
            ];
          ] ;
        ];
      ];
    ];
  ];
  sh:property [
    sh:severity s223:g36 ;
    rdfs:comment "The MultiZoneVAVAirHandlingUnit must contain a return air damper." ;
    sh:path s223:contains ;
    sh:qualifiedMinCount 1 ;
    sh:minCount 1;
    sh:qualifiedValueShape [
      sh:class g36:Damper ;
      sh:node [
        sh:property [
          sh:path s223:hasRole;
          sh:hasValue s223:Role-Return;
          sh:minCount 1;
          sh:maxCount 1;
        ];
      ];
    ] ;
  ];
  sh:property [
    sh:severity s223:g36 ;
    sh:path s223:contains;
    rdfs:comment "The  MultiZoneVAVAirHandlingUnit must contain at least one ChilledWaterCoil for cooling." ;
    sh:qualifiedMinCount 1 ;
    sh:minCount 1;
    sh:qualifiedValueShape [
      sh:class g36:ChilledWaterCoil ;
    ] ;
  ];
  sh:property [
    sh:severity s223:g36 ;
    sh:path s223:contains;
    rdfs:comment "The  MultiZoneVAVAirHandlingUnit must contain at least one HotWaterCoil or an ElectricHeatingCoil for heating." ;
    sh:qualifiedMinCount 1 ;
    sh:minCount 1;
    sh:qualifiedValueShape [
      sh:or (
        [
          sh:class g36:HotWaterCoil ;
        ]
        [
          sh:class g36:ElectricHeatingCoil ;
        ]
      );
    ] ;
  ];
.
g36:MultiZoneVAVAirHandlingUnit-AllPoints
  a sh:NodeShape, rdfs:Class, s223:Class ;
  sh:severity s223:g36;
  sh:class s223:AirHandlingUnit ;
  rdfs:subClassOf g36:MultiZoneVAVAirHandlingUnit;
  rdfs:label "MultiZoneVAVAirHandlingUnit" ;
  rdfs:comment "An assembly consisting of sections containing a fan or fans and other necessary equipment to perform one or more of the following functions: circulating, filtration, heating, cooling, heat recovery, humidifying, dehumidifying, and mixing of air. It is usually connected to an air-distribution system. This air handling unit serves multiple zones." ;
  sh:property [
    rdfs:comment "For units with a common economizer/minimum OA damper, one MultiZoneVAVAirHandlingUnit InletConnectionPoint must have at least one outdoor airflow property." ;
    sh:path s223:hasConnectionPoint;
    sh:qualifiedMinCount 1;
    sh:minCount 1;
    sh:qualifiedValueShape [
      sh:class s223:InletConnectionPoint;
      sh:node [
        sh:property [
          sh:path s223:hasProperty ;
          sh:qualifiedMinCount 1 ;
          sh:minCount 1;
          sh:qualifiedValueShape [
            sh:class s223:QuantifiableObservableProperty ;
            sh:node [
              sh:property [
                sh:path qudt:hasQuantityKind ;
                sh:hasValue quantitykind:VolumeFlowRate ;
                sh:minCount 1;
                sh:maxCount 1;
              ] ;
              sh:property [
                sh:path s223:hasAspect;
                sh:qualifiedMinCount 1;
                sh:minCount 1;
                sh:qualifiedValueShape [
                  sh:hasValue s223:Role-Outside;
                ];
              ];
            ];
          ];
        ];
      ];
    ];
  ];
  sh:property [
    sh:severity s223:g36 ;
    rdfs:comment "For units with a common economizer/minimum OA damper, it must contain a damper with the role economizer and the role outside." ;
    sh:path s223:contains ;
    sh:qualifiedMinCount 1 ;
    sh:minCount 1;
    sh:qualifiedValueShape [
      sh:class g36:Damper ;
      sh:node [
        sh:property [
          sh:path s223:hasRole;
          sh:qualifiedMinCount 1;
          sh:minCount 1 ;
          sh:qualifiedValueShape [
            sh:hasValue s223:Role-Outside;
          ];
        ];
        sh:property [
          sh:path s223:hasRole;
          sh:qualifiedMinCount 1;
          sh:minCount 1;
          sh:qualifiedValueShape [
            sh:hasValue s223:Role-Economizer;
          ];
          ];
        ];
      ];
];
  sh:property [
    sh:severity s223:g36 ;
    rdfs:comment "For units with a separate minimum outdoor air damper and DP sensor, MultiZoneVAVAirHandlingUnit must contain a two-position outdoor air damper with a differential pressure property." ;
    sh:path s223:contains ;
    sh:qualifiedMinCount 1 ;
    sh:minCount 1;
    sh:qualifiedMaxCount 1 ;
    sh:qualifiedValueShape [
      sh:class g36:TwoPositionDamper ;
      sh:node [
        sh:property [
          sh:path s223:hasRole;
          sh:qualifiedMinCount 1;
          sh:minCount 1;
          sh:qualifiedValueShape [
            sh:hasValue s223:Role-Outside;
          ];
        ];
        sh:not [
          sh:property [
            sh:path s223:hasRole;
            sh:qualifiedMinCount 1;
            sh:minCount 1 ;
            sh:qualifiedValueShape [
              sh:hasValue s223:Role-Economizer;
            ];
          ];
        ];
        sh:property [
          sh:path s223:hasProperty ;
          sh:qualifiedMinCount 1 ;
          sh:minCount 1;
          sh:qualifiedValueShape [
            sh:class s223:QuantifiableObservableProperty ;
            sh:node [
              sh:property [
                sh:path qudt:hasQuantityKind ;
                sh:hasValue quantitykind:Pressure ;
                sh:minCount 1;
                sh:maxCount 1;
              ];
            ];
          ];
        ];
      ];
    ];
  ];
  sh:property [
    sh:severity s223:g36 ;
    rdfs:comment "For units with a separate minimum outdoor air damper and AFMS, MultiZoneVAVAirHandlingUnit must contain a modulating outdoor air damper with a minimum airflow property." ;
    sh:path s223:contains ;
    sh:qualifiedMinCount 1 ;
    sh:minCount 1;
    sh:qualifiedMaxCount 1 ;
    sh:qualifiedValueShape [
      sh:class g36:Damper ;
      sh:node [
        sh:property [
          sh:path s223:hasRole;
          sh:qualifiedMinCount 1;
          sh:minCount 1;
          sh:qualifiedValueShape [
            sh:hasValue s223:Role-Outside;
          ];
        ];
        sh:not [
          sh:property [
            sh:path s223:hasRole;
            sh:qualifiedMinCount 1;
            sh:minCount 1 ;
            sh:qualifiedValueShape [
              sh:hasValue s223:Role-Economizer;
            ];
          ];
        ];
        sh:property [
          sh:path s223:hasProperty ;
          sh:qualifiedMinCount 1 ;
          sh:minCount 1;
          sh:qualifiedValueShape [
            sh:class s223:QuantifiableObservableProperty ;
            sh:node [
              sh:property [
                sh:path qudt:hasQuantityKind ;
                sh:hasValue quantitykind:VolumeFlowRate ;
                sh:minCount 1;
                sh:maxCount 1;
              ];
              sh:property [
                sh:path s223:hasAspect;
                sh:qualifiedMinCount 1;
                sh:minCount 1;
                sh:qualifiedValueShape [
                  sh:hasValue s223:Dimensioned-Minimum;
                ];
              ];
            ];
          ];
        ];
      ];
    ];
  ];
  sh:property [
    sh:severity s223:g36 ;
    rdfs:comment "For units with actuated relief dampers but no relief fan, the MultiZoneVAVAirHandlingUnit must contain a relief air damper with an analog damper command property." ;
    sh:path s223:contains ;
    sh:qualifiedMinCount 1 ;
    sh:minCount 1;
    sh:qualifiedValueShape [
      sh:class g36:Damper ;
      sh:node [
        sh:property [
          sh:path s223:hasRole;
          sh:hasValue s223:Role-Relief;
          sh:minCount 1;
          sh:maxCount 1;
        ];
      ];
    ] ;
  ];
  sh:property [
    sh:severity s223:g36 ;
    rdfs:comment "For units with actuated relief dampers but no relief fan, the MultiZoneVAVAirHandlingUnit must be connectedTo at least one VAV, which connectedTo at least one HVAC DomainSpace, which is contained by at least one Zone, which has a building static pressure property." ;
    sh:path (s223:connectedTo s223:connectedTo [sh:inversePath s223:contains;] s223:hasProperty) ;
    sh:qualifiedMinCount 1 ;
    sh:minCount 1;
    sh:qualifiedValueShape [
      sh:class s223:QuantifiableObservableProperty ;
      sh:node [
        sh:property [
          sh:path qudt:hasQuantityKind ;
          sh:hasValue quantitykind:Pressure ;
          sh:minCount 1;
          sh:maxCount 1;
        ];
      ];
    ];
  ];
  sh:property [
    sh:severity s223:g36 ;
    rdfs:comment "For units with both a relief air damper and a relief fan, the MultiZoneVAVAirHandlingUnit must have a relief air damper with a two-position damper command property." ;
    sh:path s223:contains ;
    sh:qualifiedMinCount 1 ;
    sh:minCount 1;
    sh:qualifiedMaxCount 1 ;
    sh:qualifiedValueShape [
      sh:class g36:TwoPositionDamper ;
      sh:node [
        sh:property [
          sh:path s223:hasRole;
          sh:qualifiedMinCount 1;
          sh:minCount 1;
          sh:qualifiedValueShape [
            sh:hasValue s223:Role-Relief;
          ];
        ];
      ];
    ];
  ];
  sh:property [
    sh:severity s223:g36 ;
    rdfs:comment "For units with both a relief air damper and a relief fan, the MultiZoneVAVAirHandlingUnit must have a relief fan with a VFD." ;
    sh:path s223:contains ;
    sh:qualifiedMinCount 1 ;
    sh:minCount 1;
    sh:qualifiedMaxCount 1 ;
    sh:qualifiedValueShape [
      sh:class g36:FanWithVFD ;
      sh:node [
        sh:property [
          sh:path s223:hasRole;
          sh:qualifiedMinCount 1;
          sh:minCount 1 ;
          sh:qualifiedValueShape [
            sh:hasValue s223:Role-Relief;
          ];
        ];
      ];
    ];
  ];
  sh:property [
    rdfs:comment "For units with a return fan, the MultiZoneVAVAirHandlingUnit must indeed contain a return fan." ;
    sh:severity s223:g36 ;
    sh:path s223:contains ;
    sh:qualifiedMinCount 1 ;
    sh:minCount 1;
    sh:qualifiedValueShape [
      sh:class g36:FanWithVFD ;
      sh:node [
        sh:property [
          sh:path s223:hasRole ;
          sh:hasValue s223:Role-Return ;
          sh:minCount 1 ;
        ] ;
      ] ;
    ] ;
  ] ;
  sh:property [
    sh:severity s223:g36 ;
    rdfs:comment "For units with a return fan, the MultiZoneVAVAirHandlingUnit must contain an exhaust air damper." ;
    sh:path s223:contains ;
    sh:qualifiedMinCount 1 ;
    sh:minCount 1;
    sh:qualifiedValueShape [
      sh:class g36:Damper ;
      sh:node [
        sh:property [
          sh:path s223:hasRole;
          sh:hasValue s223:Role-Exhaust;
          sh:minCount 1;
          sh:maxCount 1;
        ];
      ];
    ] ;
  ] ;
  sh:property [
    sh:severity s223:g36 ;
    rdfs:comment "For units with a return fan, if airflow tracking logic is used, the OutletConnectionPoint of the supply fan in the MultiZoneVAVAirHandlingUnit must have a supply airflow property." ;
    sh:path s223:contains ;
    sh:qualifiedMinCount 1 ;
    sh:minCount 1;
    sh:qualifiedValueShape [
      sh:class g36:FanWithVFD ;
      sh:node [
        sh:property [
          sh:path s223:hasRole ;
          sh:hasValue s223:Role-Supply ;
        ] ;
      ] ;
      sh:node [
        sh:property [
          sh:path s223:hasConnectionPoint ;
          sh:qualifiedMinCount 1 ;
          sh:minCount 1;
          sh:qualifiedValueShape [
            sh:class g36:OutletConnectionPoint ;
            sh:node [
              sh:property [
                sh:path s223:hasProperty ;
                sh:qualifiedMinCount 1;
                sh:minCount 1 ;
                sh:qualifiedValueShape [
                  sh:class s223:QuantifiableObservableProperty ;
                  sh:node [
                    sh:property [
                        sh:minCount 1 ;
                        sh:maxCount 1 ;
                        sh:path qudt:hasQuantityKind ;
                        sh:hasValue quantitykind:VolumeFlowRate ;
                    ] ;
                    sh:property [
                        sh:minCount 1 ;
                        sh:maxCount 1 ;
                        sh:path s223:hasAspect ;
                        sh:hasValue s223:Role-Supply ;
                    ] ;
                  ] ;
                ];
              ];
            ];
          ];
        ];
      ];
    ] ;
  ] ;
  sh:property [
    sh:severity s223:g36 ;
    rdfs:comment "For units with a return fan, if airflow tracking logic is used, the OutletConnectionPoint of the return fan in the MultiZoneVAVAirHandlingUnit must have a return airflow property." ;
    sh:path s223:contains ;
    sh:qualifiedMinCount 1 ;
    sh:minCount 1;
    sh:qualifiedValueShape [
      sh:class g36:FanWithVFD ;
      sh:node [
        sh:property [
          sh:path s223:hasRole ;
          sh:hasValue s223:Role-Return ;
        ] ;
      ] ;
      sh:node [
        sh:property [
          sh:path s223:hasConnectionPoint ;
          sh:qualifiedMinCount 1 ;
          sh:minCount 1;
          sh:qualifiedValueShape [
            sh:class g36:OutletConnectionPoint ;
            sh:node [
              sh:property [
                sh:path s223:hasProperty ;
                sh:qualifiedMinCount 1;
                sh:minCount 1 ;
                sh:qualifiedValueShape [
                  sh:class s223:QuantifiableObservableProperty ;
                  sh:node [
                    sh:property [
                      sh:minCount 1 ;
                      sh:maxCount 1 ;
                      sh:path qudt:hasQuantityKind ;
                      sh:hasValue quantitykind:VolumeFlowRate ;
                    ] ;
                    sh:property [
                      sh:minCount 1 ;
                      sh:maxCount 1 ;
                      sh:path s223:hasAspect ;
                      sh:hasValue s223:Role-Return ;
                    ] ;
                  ] ;
                ];
              ];
            ];
          ];
        ];
      ];
    ] ;
  ] ;
  sh:property [
    sh:severity s223:g36 ;
    rdfs:comment "For units with a return fan, if direct building pressure logic is used, the OutletConnectionPoint of the return fan in the MultiZoneVAVAirHandlingUnit must have a return fan discharge static pressure property." ;
    sh:path s223:contains ;
    sh:qualifiedMinCount 1 ;
    sh:minCount 1;
    sh:qualifiedValueShape [
      sh:class g36:FanWithVFD ;
      sh:node [
        sh:property [
          sh:path s223:hasRole ;
          sh:hasValue s223:Role-Return ;
        ] ;
      ] ;
      sh:node [
        sh:property [
          sh:path s223:hasConnectionPoint ;
          sh:qualifiedMinCount 1 ;
          sh:minCount 1;
          sh:qualifiedValueShape [
            sh:class g36:OutletConnectionPoint ;
            sh:node [
              sh:property [
                sh:path s223:hasProperty ;
                sh:qualifiedMinCount 1;
                sh:minCount 1 ;
                sh:qualifiedValueShape [
                  sh:class s223:QuantifiableObservableProperty ;
                  sh:node [
                    sh:property [
                      sh:minCount 1 ;
                      sh:maxCount 1 ;
                      sh:path qudt:hasQuantityKind ;
                      sh:hasValue quantitykind:Pressure ;
                    ] ;
                    sh:property [
                      sh:minCount 1 ;
                      sh:maxCount 1 ;
                      sh:path s223:hasAspect ;
                      sh:hasValue s223:Role-Return ;
                    ] ;
                  ] ;
                ];
              ];
            ];
          ];
        ];
      ];
    ] ;
  ] ;
  sh:property [
    sh:severity s223:g36 ;
    rdfs:comment "For units with a return fan, if direct building pressure logic is used, the MultiZoneVAVAirHandlingUnit must be connectedTo at least one VAV, which connectedTo at least one HVAC DomainSpace, which is contained by at least one Zone, which has a building static pressure property." ;
    sh:path (s223:connectedTo s223:connectedTo [sh:inversePath s223:contains;] s223:hasProperty) ;
    sh:qualifiedMinCount 1 ;
    sh:minCount 1;
    sh:qualifiedValueShape [
      sh:class s223:QuantifiableObservableProperty ;
      sh:node [
        sh:property [
          sh:path qudt:hasQuantityKind ;
          sh:hasValue quantitykind:Pressure ;
          sh:minCount 1;
          sh:maxCount 1;
        ];
      ];
    ];
  ];
.
